BigN, BigZ, BigQ: presentation via unique module with both ops and props
 We use the <+ operation to regroup all known facts about BigN
 (resp BigZ, ...) in a unique module. This uses also the new ! feature
 for controling inlining. By the way, we also make sure that these
 new BigN and BigZ modules implements OrderedTypeFull and TotalOrder,
 and also contains facts about min and max (cf. GenericMinMax).

 Side effects:
 - In NSig and ZSig, specification of compare and eq_bool is now
   done with respect to Zcompare and Zeq_bool, as for other ops.
   The order <= and < are also defined via Zle and Zlt, instead
   of using compare. Min and max are axiomatized instead of being
   macros.
 - Some proofs rework in QMake
 - QOrderedType and Qminmax were in fact not compiled by make world

 Still todo: OrderedType + MinMax for BigQ, etc etc

git-svn-id: svn+ssh://scm.gforge.inria.fr/svn/coq/trunk@12680 85f007b7-540e-0410-9357-904b9bb8a0f7

theories/Numbers/Integer/BigZ/ZMake.v
@@ -49,6 +49,7 @@ Module Make (N:NType) <: ZType.
   end.
 
  Theorem spec_of_Z: forall x, to_Z (of_Z x) = x.
+ Proof.
  intros x; case x; unfold to_Z, of_Z, zero.
    exact N.spec_0.
    intros; rewrite N.spec_of_N; auto.
@@ -85,34 +86,23 @@ Module Make (N:NType) <: ZType.
   | Neg nx, Neg ny => N.compare ny nx
   end.
 
- Definition lt n m := compare n m = Lt.
- Definition le n m := compare n m <> Gt.
- Definition min n m := match compare n m with Gt => m | _ => n end.
- Definition max n m := match compare n m with Lt => m | _ => n end.
-
- Theorem spec_compare: forall x y,
-    match compare x y with
-      Eq => to_Z x = to_Z y
-    | Lt => to_Z x < to_Z y
-    | Gt => to_Z x > to_Z y
-    end.
-  unfold compare, to_Z; intros x y; case x; case y; clear x y;
-    intros x y; auto; generalize (N.spec_pos x) (N.spec_pos y).
-  generalize (N.spec_compare y x); case N.compare; auto with zarith.
-  generalize (N.spec_compare y N.zero); case N.compare;
-     try rewrite N.spec_0; auto with zarith.
-  generalize (N.spec_compare x N.zero); case N.compare;
-   rewrite N.spec_0; auto with zarith.
-  generalize (N.spec_compare x N.zero); case N.compare;
-   rewrite N.spec_0; auto with zarith.
-  generalize (N.spec_compare N.zero y); case N.compare;
-     try rewrite N.spec_0; auto with zarith.
-  generalize (N.spec_compare N.zero x); case N.compare;
-   rewrite N.spec_0; auto with zarith.
-  generalize (N.spec_compare N.zero x); case N.compare;
-   rewrite N.spec_0; auto with zarith.
-  generalize (N.spec_compare x y); case N.compare; auto with zarith.
-  Qed.
+ Theorem spec_compare :
+  forall x y, compare x y = Zcompare (to_Z x) (to_Z y).
+ Proof.
+ unfold compare, to_Z.
+ destruct x as [x|x], y as [y|y];
+ rewrite ?N.spec_compare, ?N.spec_0, <-?Zcompare_opp; auto;
+ assert (Hx:=N.spec_pos x); assert (Hy:=N.spec_pos y);
+ set (X:=N.to_Z x) in *; set (Y:=N.to_Z y) in *; clearbody X Y.
+ destruct (Zcompare_spec X 0) as [EQ|LT|GT].
+  rewrite EQ. rewrite <- Zopp_0 at 2. apply Zcompare_opp.
+  exfalso. omega.
+  symmetry. change (X > -Y). omega.
+ destruct (Zcompare_spec 0 X) as [EQ|LT|GT].
+  rewrite <- EQ. rewrite Zopp_0; auto.
+  symmetry. change (-X < Y). omega.
+  exfalso. omega.
+ Qed.
 
  Definition eq_bool x y :=
   match compare x y with
@@ -120,36 +110,27 @@ Module Make (N:NType) <: ZType.
   | _ => false
   end.
 
- Theorem spec_eq_bool: forall x y,
-    if eq_bool x y then to_Z x = to_Z y else to_Z x <> to_Z y.
- intros x y; unfold eq_bool;
-   generalize (spec_compare x y); case compare; auto with zarith.
+ Theorem spec_eq_bool:
+  forall x y, eq_bool x y = Zeq_bool (to_Z x) (to_Z y).
+ Proof.
+ unfold eq_bool, Zeq_bool; intros; rewrite spec_compare; reflexivity.
  Qed.
 
- Definition cmp_sign x y :=
-  match x, y with
-  | Pos nx, Neg ny =>
-    if N.eq_bool ny N.zero then Eq else Gt
-  | Neg nx, Pos ny =>
-    if N.eq_bool nx N.zero then Eq else Lt
-  | _, _ => Eq
-  end.
+ Definition lt n m := to_Z n < to_Z m.
+ Definition le n m := to_Z n <= to_Z m.
 
- Theorem spec_cmp_sign: forall x y,
-  match cmp_sign x y with
-  | Gt => 0 <= to_Z x /\ to_Z y < 0
-  | Lt => to_Z x <  0 /\ 0 <= to_Z y
-  | Eq => True
-  end.
-  Proof.
-  intros [x | x] [y | y]; unfold cmp_sign; auto.
-  generalize (N.spec_eq_bool y N.zero); case N.eq_bool; auto.
-  rewrite N.spec_0; unfold to_Z.
-  generalize (N.spec_pos x) (N.spec_pos y); auto with zarith.
-  generalize (N.spec_eq_bool x N.zero); case N.eq_bool; auto.
-  rewrite N.spec_0; unfold to_Z.
-  generalize (N.spec_pos x) (N.spec_pos y); auto with zarith.
-  Qed.
+ Definition min n m := match compare n m with Gt => m | _ => n end.
+ Definition max n m := match compare n m with Lt => m | _ => n end.
+
+ Theorem spec_min : forall n m, to_Z (min n m) = Zmin (to_Z n) (to_Z m).
+ Proof.
+ unfold min, Zmin. intros. rewrite spec_compare. destruct Zcompare; auto.
+ Qed.
+
+ Theorem spec_max : forall n m, to_Z (max n m) = Zmax (to_Z n) (to_Z m).
+ Proof.
+ unfold max, Zmax. intros. rewrite spec_compare. destruct Zcompare; auto.
+ Qed.
 
  Definition to_N x :=
   match x with
@@ -160,6 +141,7 @@ Module Make (N:NType) <: ZType.
  Definition abs x := Pos (to_N x).
 
  Theorem spec_abs: forall x, to_Z (abs x) = Zabs (to_Z x).
+ Proof.
  intros x; case x; clear x; intros x; assert (F:=N.spec_pos x).
     simpl; rewrite Zabs_eq; auto.
  simpl; rewrite Zabs_non_eq; simpl; auto with zarith.
@@ -172,6 +154,7 @@ Module Make (N:NType) <: ZType.
   end.
 
  Theorem spec_opp: forall x, to_Z (opp x) = - to_Z x.
+ Proof.
  intros x; case x; simpl; auto with zarith.
  Qed.
 
@@ -186,10 +169,10 @@ Module Make (N:NType) <: ZType.
   end.
 
  Theorem spec_succ: forall n, to_Z (succ n) = to_Z n + 1.
+ Proof.
  intros x; case x; clear x; intros x.
    exact (N.spec_succ x).
- simpl; generalize (N.spec_compare N.zero x); case N.compare;
-   rewrite N.spec_0; simpl.
+ simpl. rewrite N.spec_compare. case Zcompare_spec; rewrite ?N.spec_0; simpl.
   intros HH; rewrite <- HH; rewrite N.spec_1; ring.
   intros HH; rewrite N.spec_pred, Zmax_r; auto with zarith.
  generalize (N.spec_pos x); auto with zarith.
@@ -214,17 +197,11 @@ Module Make (N:NType) <: ZType.
   end.
 
  Theorem spec_add: forall x y, to_Z (add x y) = to_Z x +  to_Z y.
- unfold add, to_Z; intros [x | x] [y | y].
-   exact (N.spec_add x y).
- unfold zero; generalize (N.spec_compare x y); case N.compare.
-   rewrite N.spec_0; auto with zarith.
- intros; rewrite N.spec_sub, Zmax_r; auto with zarith.
- intros; rewrite N.spec_sub, Zmax_r; auto with zarith.
- unfold zero; generalize (N.spec_compare x y); case N.compare.
-   rewrite N.spec_0; auto with zarith.
- intros; rewrite N.spec_sub, Zmax_r; auto with zarith.
- intros; rewrite N.spec_sub, Zmax_r; auto with zarith.
- intros; rewrite N.spec_add; auto with zarith.
+ Proof.
+ unfold add, to_Z; intros [x | x] [y | y];
+   try (rewrite N.spec_add; auto with zarith);
+ rewrite N.spec_compare; case Zcompare_spec;
+  unfold zero; rewrite ?N.spec_0, ?N.spec_sub; omega with *.
  Qed.
 
  Definition pred x :=
@@ -238,12 +215,12 @@ Module Make (N:NType) <: ZType.
   end.
 
  Theorem spec_pred: forall x, to_Z (pred x) = to_Z x - 1.
- unfold pred, to_Z, minus_one; intros [x | x].
-   generalize (N.spec_compare N.zero x); case N.compare;
-     rewrite N.spec_0; try rewrite N.spec_1; auto with zarith.
-   intros H; rewrite N.spec_pred, Zmax_r; auto with zarith.
- generalize (N.spec_pos x); auto with zarith.
- rewrite N.spec_succ; ring.
+ Proof.
+ unfold pred, to_Z, minus_one; intros [x | x];
+   try (rewrite N.spec_succ; ring).
+ rewrite N.spec_compare; case Zcompare_spec;
+  rewrite ?N.spec_0, ?N.spec_1, ?N.spec_pred;
+  generalize (N.spec_pos x); omega with *.
  Qed.
 
  Definition sub x y :=
@@ -265,17 +242,11 @@ Module Make (N:NType) <: ZType.
   end.
 
  Theorem spec_sub: forall x y, to_Z (sub x y) = to_Z x - to_Z y.
- unfold sub, to_Z; intros [x | x] [y | y].
- unfold zero; generalize (N.spec_compare x y); case N.compare.
-   rewrite N.spec_0; auto with zarith.
- intros; rewrite N.spec_sub, Zmax_r; auto with zarith.
- intros; rewrite N.spec_sub, Zmax_r; auto with zarith.
- rewrite N.spec_add; auto with zarith.
- rewrite N.spec_add; auto with zarith.
- unfold zero; generalize (N.spec_compare x y); case N.compare.
-   rewrite N.spec_0; auto with zarith.
- intros; rewrite N.spec_sub, Zmax_r; auto with zarith.
- intros; rewrite N.spec_sub, Zmax_r; auto with zarith.
+ Proof.
+ unfold sub, to_Z; intros [x | x] [y | y];
+  try (rewrite N.spec_add; auto with zarith);
+ rewrite N.spec_compare; case Zcompare_spec;
+  unfold zero; rewrite ?N.spec_0, ?N.spec_sub; omega with *.
  Qed.
 
  Definition mul x y :=
@@ -286,8 +257,8 @@ Module Make (N:NType) <: ZType.
   | Neg nx, Neg ny => Pos (N.mul nx ny)
   end.
 
-
  Theorem spec_mul: forall x y, to_Z (mul x y) = to_Z x * to_Z y.
+ Proof.
  unfold mul, to_Z; intros [x | x] [y | y]; rewrite N.spec_mul; ring.
  Qed.
 
@@ -298,6 +269,7 @@ Module Make (N:NType) <: ZType.
   end.
 
  Theorem spec_square: forall x, to_Z (square x) = to_Z x *  to_Z x.
+ Proof.
  unfold square, to_Z; intros [x | x]; rewrite N.spec_square; ring.
  Qed.
 
@@ -313,6 +285,7 @@ Module Make (N:NType) <: ZType.
   end.
 
  Theorem spec_power_pos: forall x n, to_Z (power_pos x n) = to_Z x ^ Zpos n.
+ Proof.
  assert (F0: forall x, (-x)^2 = x^2).
    intros x; rewrite Zpower_2; ring.
  unfold power_pos, to_Z; intros [x | x] [p | p |];
@@ -335,9 +308,9 @@ Module Make (N:NType) <: ZType.
   | Neg nx => Neg N.zero
   end.
 
-
  Theorem spec_sqrt: forall x, 0 <= to_Z x ->
    to_Z (sqrt x) ^ 2 <= to_Z x < (to_Z (sqrt x) + 1) ^ 2.
+ Proof.
  unfold to_Z, sqrt; intros [x | x] H.
    exact (N.spec_sqrt x).
  replace (N.to_Z x) with 0.
@@ -353,144 +326,74 @@ Module Make (N:NType) <: ZType.
     (Pos q, Pos r)
   | Pos nx, Neg ny =>
     let (q, r) := N.div_eucl nx ny in
-    match N.compare N.zero r with
-    | Eq => (Neg q, zero)
-    | _ => (Neg (N.succ q), Neg (N.sub ny r))
-    end
+    if N.eq_bool N.zero r
+    then (Neg q, zero)
+    else (Neg (N.succ q), Neg (N.sub ny r))
   | Neg nx, Pos ny =>
     let (q, r) := N.div_eucl nx ny in
-    match N.compare N.zero r with
-    | Eq => (Neg q, zero)
-    | _ => (Neg (N.succ q), Pos (N.sub ny r))
-    end
+    if N.eq_bool N.zero r
+    then (Neg q, zero)
+    else (Neg (N.succ q), Pos (N.sub ny r))
   | Neg nx, Neg ny =>
     let (q, r) := N.div_eucl nx ny in
     (Pos q, Neg r)
   end.
 
-
- Theorem spec_div_eucl_nz: forall x y,
-      to_Z y <> 0 ->
-      let (q,r) := div_eucl x y in
-      (to_Z q, to_Z r) = Zdiv_eucl (to_Z x) (to_Z y).
- unfold div_eucl, to_Z; intros [x | x] [y | y] H.
- assert (H1: 0 < N.to_Z y).
-   generalize (N.spec_pos y); auto with zarith.
- generalize (N.spec_div_eucl x y); case N.div_eucl; auto.
- assert (HH: 0 < N.to_Z y).
-   generalize (N.spec_pos y); auto with zarith.
- generalize (N.spec_div_eucl x y); case N.div_eucl; auto.
- intros q r; generalize (N.spec_pos x) HH; unfold Zdiv_eucl;
-   case_eq (N.to_Z x); case_eq (N.to_Z y);
-     try (intros; apply False_ind; auto with zarith; fail).
- intros p He1 He2 _ _ H1; injection H1; intros H2 H3.
- generalize (N.spec_compare N.zero r); case N.compare;
-   unfold zero; rewrite N.spec_0; try rewrite H3; auto.
- rewrite H2; intros; apply False_ind; auto with zarith.
- rewrite H2; intros; apply False_ind; auto with zarith.
- intros p _ _ _ H1; discriminate H1.
- intros p He p1 He1 H1 _.
- generalize (N.spec_compare N.zero r); case N.compare.
- change (- Zpos p) with (Zneg p).
- unfold zero; lazy zeta.
- rewrite N.spec_0; intros H2; rewrite <- H2.
- intros H3; rewrite <- H3; auto.
- rewrite N.spec_0; intros H2.
- change (- Zpos p) with (Zneg p); lazy iota beta.
- intros H3; rewrite <- H3; auto.
- rewrite N.spec_succ; rewrite N.spec_sub, Zmax_r.
- generalize H2; case (N.to_Z r).
- intros; apply False_ind; auto with zarith.
- intros p2 _; rewrite He; auto with zarith.
- change (Zneg p) with (- (Zpos p)); apply f_equal2 with (f := @pair Z Z); ring.
- intros p2 H4; discriminate H4.
- assert (N.to_Z r = (Zpos p1 mod (Zpos p))).
-   unfold Zmod, Zdiv_eucl; rewrite <- H3; auto.
- case (Z_mod_lt (Zpos p1) (Zpos p)); auto with zarith.
- rewrite N.spec_0; intros H2; generalize (N.spec_pos r);
-   intros; apply False_ind; auto with zarith.
- assert (HH: 0 < N.to_Z y).
-   generalize (N.spec_pos y); auto with zarith.
- generalize (N.spec_div_eucl x y); case N.div_eucl; auto.
- intros q r; generalize (N.spec_pos x) HH; unfold Zdiv_eucl;
-   case_eq (N.to_Z x); case_eq (N.to_Z y);
-     try (intros; apply False_ind; auto with zarith; fail).
- intros p He1 He2 _ _ H1; injection H1; intros H2 H3.
- generalize (N.spec_compare N.zero r); case N.compare;
-   unfold zero; rewrite N.spec_0; try rewrite H3; auto.
- rewrite H2; intros; apply False_ind; auto with zarith.
- rewrite H2; intros; apply False_ind; auto with zarith.
- intros p _ _ _ H1; discriminate H1.
- intros p He p1 He1 H1 _.
- generalize (N.spec_compare N.zero r); case N.compare.
- change (- Zpos p1) with (Zneg p1).
- unfold zero; lazy zeta.
- rewrite N.spec_0; intros H2; rewrite <- H2.
- intros H3; rewrite <- H3; auto.
- rewrite N.spec_0; intros H2.
- change (- Zpos p1) with (Zneg p1); lazy iota beta.
- intros H3; rewrite <- H3; auto.
- rewrite N.spec_succ; rewrite N.spec_sub, Zmax_r.
- generalize H2; case (N.to_Z r).
- intros; apply False_ind; auto with zarith.
- intros p2 _; rewrite He; auto with zarith.
- intros p2 H4; discriminate H4.
- assert (N.to_Z r = (Zpos p1 mod (Zpos p))).
-   unfold Zmod, Zdiv_eucl; rewrite <- H3; auto.
- case (Z_mod_lt (Zpos p1) (Zpos p)); auto with zarith.
- rewrite N.spec_0; generalize (N.spec_pos r); intros; apply False_ind; auto with zarith.
- assert (H1: 0 < N.to_Z y).
-   generalize (N.spec_pos y); auto with zarith.
- generalize (N.spec_div_eucl x y); case N.div_eucl; auto.
- intros q r; generalize (N.spec_pos x) H1; unfold Zdiv_eucl;
-   case_eq (N.to_Z x); case_eq (N.to_Z y);
-     try (intros; apply False_ind; auto with zarith; fail).
- change (-0) with 0; lazy iota beta; auto.
- intros p _ _ _ _ H2; injection H2.
- intros H3 H4; rewrite H3; rewrite H4; auto.
- intros p _ _ _ H2; discriminate H2.
- intros p He p1 He1 _ _  H2.
- change (- Zpos p1) with (Zneg p1); lazy iota beta.
- change (- Zpos p) with (Zneg p); lazy iota beta.
- rewrite <- H2; auto.
- Qed.
-
- Lemma Zdiv_eucl_0 : forall a, Zdiv_eucl a 0 = (0,0).
- Proof. destruct a; auto. Qed.
+ Ltac break_nonneg x px EQx :=
+  let H := fresh "H" in
+  assert (H:=N.spec_pos x);
+  destruct (N.to_Z x) as [|px|px]_eqn:EQx;
+   [clear H|clear H|elim H; reflexivity].
 
  Theorem spec_div_eucl: forall x y,
-      let (q,r) := div_eucl x y in
-      (to_Z q, to_Z r) = Zdiv_eucl (to_Z x) (to_Z y).
+   let (q,r) := div_eucl x y in
+   (to_Z q, to_Z r) = Zdiv_eucl (to_Z x) (to_Z y).
  Proof.
- intros. destruct (Z_eq_dec (to_Z y) 0) as [EQ|NEQ];
-  [|apply spec_div_eucl_nz; auto].
- unfold div_eucl.
- destruct x; destruct y; simpl in *.
- generalize (N.spec_div_eucl t0 t1). destruct N.div_eucl; simpl; auto.
- generalize (N.spec_div_eucl t0 t1). destruct N.div_eucl; simpl; auto.
- assert (EQ' : N.to_Z t1 = 0) by auto with zarith.
- rewrite EQ'. simpl. rewrite Zdiv_eucl_0. injection 1; intros.
- generalize (N.spec_compare N.zero t3); destruct N.compare.
- simpl. intros. f_equal; auto with zarith.
- rewrite N.spec_0; intro; exfalso; auto with zarith.
- rewrite N.spec_0; intro; exfalso; auto with zarith.
- generalize (N.spec_div_eucl t0 t1). destruct N.div_eucl; simpl; auto.
- assert (EQ' : N.to_Z t1 = 0) by auto with zarith.
- rewrite EQ'. simpl. rewrite 2 Zdiv_eucl_0. injection 1; intros.
- generalize (N.spec_compare N.zero t3); destruct N.compare.
- simpl. intros. f_equal; auto with zarith.
- rewrite N.spec_0; intro; exfalso; auto with zarith.
- rewrite N.spec_0; intro; exfalso; auto with zarith.
- generalize (N.spec_div_eucl t0 t1). destruct N.div_eucl; simpl; auto.
- assert (EQ' : N.to_Z t1 = 0) by auto with zarith.
- rewrite EQ'. simpl. rewrite 2 Zdiv_eucl_0. injection 1; intros.
- f_equal; auto with zarith.
+ unfold div_eucl, to_Z. intros [x | x] [y | y].
+ (* Pos Pos *)
+ generalize (N.spec_div_eucl x y); destruct (N.div_eucl x y); auto.
+ (* Pos Neg *)
+ generalize (N.spec_div_eucl x y); destruct (N.div_eucl x y) as (q,r).
+ break_nonneg x px EQx; break_nonneg y py EQy;
+ try (injection 1; intros Hr Hq; rewrite N.spec_eq_bool, N.spec_0, Hr;
+      simpl; rewrite Hq, N.spec_0; auto).
+ change (- Zpos py) with (Zneg py).
+ assert (GT : Zpos py > 0) by (compute; auto).
+ generalize (Z_div_mod (Zpos px) (Zpos py) GT).
+ unfold Zdiv_eucl. destruct (Zdiv_eucl_POS px (Zpos py)) as (q',r').
+ intros (EQ,MOD). injection 1. intros Hr' Hq'.
+ rewrite N.spec_eq_bool, N.spec_0, Hr'.
+ break_nonneg r pr EQr.
+ subst; simpl. rewrite N.spec_0; auto.
+ subst. lazy iota beta delta [Zeq_bool Zcompare].
+ rewrite N.spec_sub, N.spec_succ, EQy, EQr. f_equal. omega with *.
+ (* Neg Pos *)
+ generalize (N.spec_div_eucl x y); destruct (N.div_eucl x y) as (q,r).
+ break_nonneg x px EQx; break_nonneg y py EQy;
+ try (injection 1; intros Hr Hq; rewrite N.spec_eq_bool, N.spec_0, Hr;
+      simpl; rewrite Hq, N.spec_0; auto).
+ change (- Zpos px) with (Zneg px).
+ assert (GT : Zpos py > 0) by (compute; auto).
+ generalize (Z_div_mod (Zpos px) (Zpos py) GT).
+ unfold Zdiv_eucl. destruct (Zdiv_eucl_POS px (Zpos py)) as (q',r').
+ intros (EQ,MOD). injection 1. intros Hr' Hq'.
+ rewrite N.spec_eq_bool, N.spec_0, Hr'.
+ break_nonneg r pr EQr.
+ subst; simpl. rewrite N.spec_0; auto.
+ subst. lazy iota beta delta [Zeq_bool Zcompare].
+ rewrite N.spec_sub, N.spec_succ, EQy, EQr. f_equal. omega with *.
+ (* Neg Neg *)
+ generalize (N.spec_div_eucl x y); destruct (N.div_eucl x y) as (q,r).
+ break_nonneg x px EQx; break_nonneg y py EQy;
+ try (injection 1; intros Hr Hq; rewrite Hr, Hq; auto).
+ simpl. intros <-; auto.
  Qed.
 
  Definition div x y := fst (div_eucl x y).
 
  Definition spec_div: forall x y,
      to_Z (div x y) = to_Z x / to_Z y.
+ Proof.
  intros x y; generalize (spec_div_eucl x y); unfold div, Zdiv.
  case div_eucl; case Zdiv_eucl; simpl; auto.
  intros q r q11 r1 H; injection H; auto.
@@ -500,6 +403,7 @@ Module Make (N:NType) <: ZType.
 
  Theorem spec_modulo:
    forall x y, to_Z (modulo x y) = to_Z x mod to_Z y.
+ Proof.
  intros x y; generalize (spec_div_eucl x y); unfold modulo, Zmod.
  case div_eucl; case Zdiv_eucl; simpl; auto.
  intros q r q11 r1 H; injection H; auto.
@@ -514,6 +418,7 @@ Module Make (N:NType) <: ZType.
   end.
 
  Theorem spec_gcd: forall a b, to_Z (gcd a b) = Zgcd (to_Z a) (to_Z b).
+ Proof.
  unfold gcd, Zgcd, to_Z; intros [x | x] [y | y]; rewrite N.spec_gcd; unfold Zgcd;
   auto; case N.to_Z; simpl; auto with zarith;
   try rewrite Zabs_Zopp; auto;
@@ -529,8 +434,7 @@ Module Make (N:NType) <: ZType.
 
  Lemma spec_sgn : forall x, to_Z (sgn x) = Zsgn (to_Z x).
  Proof.
- intros. unfold sgn. generalize (spec_compare zero x).
- destruct compare.
+ intros. unfold sgn. rewrite spec_compare. case Zcompare_spec.
  rewrite spec_0. intros <-; auto.
  rewrite spec_0, spec_1. symmetry. rewrite Zsgn_pos; auto.
  rewrite spec_0, spec_m1. symmetry. rewrite Zsgn_neg; auto with zarith.
