theories/Numbers/Integer/SpecViaZ/ZSig.v
@@ -25,100 +25,75 @@ Module Type ZType.
  Parameter t : Type.
 
  Parameter to_Z : t -> Z.
- Notation "[ x ]" := (to_Z x).
+ Local Notation "[ x ]" := (to_Z x).
 
- Definition eq x y := ([x] = [y]).
+ Definition eq x y := [x] = [y].
+ Definition lt x y := [x] < [y].
+ Definition le x y := [x] <= [y].
 
  Parameter of_Z : Z -> t.
  Parameter spec_of_Z: forall x, to_Z (of_Z x) = x.
 
+ Parameter compare : t -> t -> comparison.
+ Parameter eq_bool : t -> t -> bool.
+ Parameter min : t -> t -> t.
+ Parameter max : t -> t -> t.
  Parameter zero : t.
  Parameter one : t.
  Parameter minus_one : t.
+ Parameter succ : t -> t.
+ Parameter add  : t -> t -> t.
+ Parameter pred : t -> t.
+ Parameter sub : t -> t -> t.
+ Parameter opp : t -> t.
+ Parameter mul : t -> t -> t.
+ Parameter square : t -> t.
+ Parameter power_pos : t -> positive -> t.
+ Parameter sqrt : t -> t.
+ Parameter div_eucl : t -> t -> t * t.
+ Parameter div : t -> t -> t.
+ Parameter modulo : t -> t -> t.
+ Parameter gcd : t -> t -> t.
+ Parameter sgn : t -> t.
+ Parameter abs : t -> t.
 
+ Parameter spec_compare: forall x y, compare x y = Zcompare [x] [y].
+ Parameter spec_eq_bool: forall x y, eq_bool x y = Zeq_bool [x] [y].
+ Parameter spec_min : forall x y, [min x y] = Zmin [x] [y].
+ Parameter spec_max : forall x y, [max x y] = Zmax [x] [y].
  Parameter spec_0: [zero] = 0.
  Parameter spec_1: [one] = 1.
  Parameter spec_m1: [minus_one] = -1.
-
- Parameter compare : t -> t -> comparison.
-
- Parameter spec_compare: forall x y,
-   match compare x y with
-     | Eq => [x] = [y]
-     | Lt => [x] < [y]
-     | Gt => [x] > [y]
-   end.
-
- Definition lt n m := compare n m = Lt.
- Definition le n m := compare n m <> Gt.
- Definition min n m := match compare n m with Gt => m | _ => n end.
- Definition max n m := match compare n m with Lt => m | _ => n end.
-
- Parameter eq_bool : t -> t -> bool.
-
- Parameter spec_eq_bool: forall x y,
-    if eq_bool x y then [x] = [y] else [x] <> [y].
-
- Parameter succ : t -> t.
-
  Parameter spec_succ: forall n, [succ n] = [n] + 1.
-
- Parameter add  : t -> t -> t.
-
  Parameter spec_add: forall x y, [add x y] = [x] + [y].
-
- Parameter pred : t -> t.
-
  Parameter spec_pred: forall x, [pred x] = [x] - 1.
-
- Parameter sub : t -> t -> t.
-
  Parameter spec_sub: forall x y, [sub x y] = [x] - [y].
-
- Parameter opp : t -> t.
-
  Parameter spec_opp: forall x, [opp x] = - [x].
-
- Parameter mul : t -> t -> t.
-
  Parameter spec_mul: forall x y, [mul x y] = [x] * [y].
-
- Parameter square : t -> t.
-
  Parameter spec_square: forall x, [square x] = [x] *  [x].
-
- Parameter power_pos : t -> positive -> t.
-
  Parameter spec_power_pos: forall x n, [power_pos x n] = [x] ^ Zpos n.
-
- Parameter sqrt : t -> t.
-
  Parameter spec_sqrt: forall x, 0 <= [x] ->
    [sqrt x] ^ 2 <= [x] < ([sqrt x] + 1) ^ 2.
-
- Parameter div_eucl : t -> t -> t * t.
-
  Parameter spec_div_eucl: forall x y,
    let (q,r) := div_eucl x y in ([q], [r]) = Zdiv_eucl [x] [y].
-
- Parameter div : t -> t -> t.
-
  Parameter spec_div: forall x y, [div x y] = [x] / [y].
-
- Parameter modulo : t -> t -> t.
-
  Parameter spec_modulo: forall x y, [modulo x y] = [x] mod [y].
-
- Parameter gcd : t -> t -> t.
-
  Parameter spec_gcd: forall a b, [gcd a b] = Zgcd (to_Z a) (to_Z b).
-
- Parameter sgn : t -> t.
-
  Parameter spec_sgn : forall x, [sgn x] = Zsgn [x].
-
- Parameter abs : t -> t.
-
  Parameter spec_abs : forall x, [abs x] = Zabs [x].
 
 End ZType.
+
+Module Type ZType_Notation (Import Z:ZType).
+ Notation "[ x ]" := (to_Z x).
+ Infix "=="  := eq (at level 70).
+ Notation "0" := zero.
+ Infix "+" := add.
+ Infix "-" := sub.
+ Infix "*" := mul.
+ Notation "- x" := (opp x).
+ Infix "<=" := le.
+ Infix "<" := lt.
+End ZType_Notation.
+
+Module Type ZType' := ZType <+ ZType_Notation.
