theories/Numbers/Natural/SpecViaZ/NSig.v
@@ -25,87 +25,67 @@ Module Type NType.
  Parameter t : Type.
 
  Parameter to_Z : t -> Z.
- Notation "[ x ]" := (to_Z x).
+ Local Notation "[ x ]" := (to_Z x).
  Parameter spec_pos: forall x, 0 <= [x].
 
  Parameter of_N : N -> t.
  Parameter spec_of_N: forall x, to_Z (of_N x) = Z_of_N x.
  Definition to_N n := Zabs_N (to_Z n).
 
- Definition eq n m := ([n] = [m]).
-
- Parameter zero : t.
- Parameter one : t.
-
- Parameter spec_0: [zero] = 0.
- Parameter spec_1: [one] = 1.
+ Definition eq n m := [n] = [m].
+ Definition lt n m := [n] < [m].
+ Definition le n m := [n] <= [m].
 
  Parameter compare : t -> t -> comparison.
-
- Parameter spec_compare: forall x y,
-   match compare x y with
-     | Eq => [x] = [y]
-     | Lt => [x] < [y]
-     | Gt => [x] > [y]
-   end.
-
- Definition lt n m := compare n m = Lt.
- Definition le n m := compare n m <> Gt.
- Definition min n m := match compare n m with Gt => m | _ => n end.
- Definition max n m := match compare n m with Lt => m | _ => n end.
-
  Parameter eq_bool : t -> t -> bool.
-
- Parameter spec_eq_bool: forall x y,
-    if eq_bool x y then [x] = [y] else [x] <> [y].
-
+ Parameter max : t -> t -> t.
+ Parameter min : t -> t -> t.
+ Parameter zero : t.
+ Parameter one : t.
  Parameter succ : t -> t.
-
- Parameter spec_succ: forall n, [succ n] = [n] + 1.
-
- Parameter add  : t -> t -> t.
-
- Parameter spec_add: forall x y, [add x y] = [x] + [y].
-
  Parameter pred : t -> t.
-
- Parameter spec_pred: forall x, [pred x] = Zmax 0 ([x] - 1).
-
+ Parameter add  : t -> t -> t.
  Parameter sub : t -> t -> t.
-
- Parameter spec_sub: forall x y, [sub x y] = Zmax 0 ([x] - [y]).
-
  Parameter mul : t -> t -> t.
-
- Parameter spec_mul: forall x y, [mul x y] = [x] * [y].
-
  Parameter square : t -> t.
-
- Parameter spec_square: forall x, [square x] = [x] *  [x].
-
  Parameter power_pos : t -> positive -> t.
-
- Parameter spec_power_pos: forall x n, [power_pos x n] = [x] ^ Zpos n.
-
  Parameter sqrt : t -> t.
-
- Parameter spec_sqrt: forall x, [sqrt x] ^ 2 <= [x] < ([sqrt x] + 1) ^ 2.
-
  Parameter div_eucl : t -> t -> t * t.
-
- Parameter spec_div_eucl: forall x y,
-  let (q,r) := div_eucl x y in ([q], [r]) = Zdiv_eucl [x] [y].
-
  Parameter div : t -> t -> t.
-
- Parameter spec_div: forall x y, [div x y] = [x] / [y].
-
  Parameter modulo : t -> t -> t.
-
- Parameter spec_modulo: forall x y, [modulo x y] = [x] mod [y].
-
  Parameter gcd : t -> t -> t.
 
- Parameter spec_gcd: forall a b, [gcd a b] = Zgcd (to_Z a) (to_Z b).
+ Parameter spec_compare: forall x y, compare x y = Zcompare [x] [y].
+ Parameter spec_eq_bool: forall x y, eq_bool x y = Zeq_bool [x] [y].
+ Parameter spec_max : forall x y, [max x y] = Zmax [x] [y].
+ Parameter spec_min : forall x y, [min x y] = Zmin [x] [y].
+ Parameter spec_0: [zero] = 0.
+ Parameter spec_1: [one] = 1.
+ Parameter spec_succ: forall n, [succ n] = [n] + 1.
+ Parameter spec_add: forall x y, [add x y] = [x] + [y].
+ Parameter spec_pred: forall x, [pred x] = Zmax 0 ([x] - 1).
+ Parameter spec_sub: forall x y, [sub x y] = Zmax 0 ([x] - [y]).
+ Parameter spec_mul: forall x y, [mul x y] = [x] * [y].
+ Parameter spec_square: forall x, [square x] = [x] *  [x].
+ Parameter spec_power_pos: forall x n, [power_pos x n] = [x] ^ Zpos n.
+ Parameter spec_sqrt: forall x, [sqrt x] ^ 2 <= [x] < ([sqrt x] + 1) ^ 2.
+ Parameter spec_div_eucl: forall x y,
+  let (q,r) := div_eucl x y in ([q], [r]) = Zdiv_eucl [x] [y].
+ Parameter spec_div: forall x y, [div x y] = [x] / [y].
+ Parameter spec_modulo: forall x y, [modulo x y] = [x] mod [y].
+ Parameter spec_gcd: forall a b, [gcd a b] = Zgcd [a] [b].
 
 End NType.
+
+Module Type NType_Notation (Import N:NType).
+ Notation "[ x ]" := (to_Z x).
+ Infix "==" := eq (at level 70).
+ Notation "0" := zero.
+ Infix "+" := add.
+ Infix "-" := sub.
+ Infix "*" := mul.
+ Infix "<=" := le.
+ Infix "<" := lt.
+End NType_Notation.
+
+Module Type NType' := NType <+ NType_Notation.
